code/poly1305/Hacl.Spec.Poly1305.Vec.fst
@@ -1,7 +1,5 @@
 module Hacl.Spec.Poly1305.Vec
 
-#reset-options "--z3rlimit 60 --initial_fuel 0 --max_fuel 0 --initial_ifuel 0 --max_ifuel 0"
-
 open FStar.Mul
 open Lib.IntTypes
 open Lib.Sequence
@@ -10,9 +8,10 @@ open Lib.IntVector
 
 module Scalar = Spec.Poly1305
 
+#reset-options "--z3rlimit 50 --max_fuel 0 --max_ifuel 0"
+
 (* Field types and parameters *)
-val lemma_pow2_128: n:nat ->
-  Lemma
+val lemma_pow2_128: n:nat -> Lemma
   (requires n <= 128)
   (ensures pow2 n < Scalar.prime)
   [SMTPat (pow2 n)]
@@ -26,7 +25,7 @@ let pfelem = Scalar.felem
 let pfadd (x:pfelem) (y:pfelem) : pfelem = Scalar.fadd x y
 let pfmul (x:pfelem) (y:pfelem) : pfelem = Scalar.fmul x y
 
-let lanes = w:width{w == 1 \/ w == 2 \/ w == 4}
+let lanes = w:width{w == 1 \/ w == 2 \/ w == 4 \/ w == 8}
 type elem (w:lanes) = lseq pfelem w
 
 
@@ -42,81 +41,78 @@ let fmul (#w:lanes) (x:elem w) (y:elem w) : elem w =
 (* Specification *)
 let size_block : size_nat = Scalar.size_block
 
-let load_elem1 (b:Scalar.block) : elem 1 =
-  to_elem 1 (nat_from_bytes_le b)
-
-let load_elem2 (b:lbytes (2 * size_block)) : elem 2 =
-  let b1 = nat_from_bytes_le (sub b 0 size_block) in
-  let b2 = nat_from_bytes_le (sub b size_block size_block) in
-  create2 b1 b2
-
-let load_elem4 (b:lbytes (4 * size_block)) : elem 4 =
-  let b1 = nat_from_bytes_le (sub b 0 size_block) in
-  let b2 = nat_from_bytes_le (sub b size_block size_block) in
-  let b3 = nat_from_bytes_le (sub b (2 * size_block) size_block) in
-  let b4 = nat_from_bytes_le (sub b (3 * size_block) size_block) in
-  create4 b1 b2 b3 b4
+let load_elem1 (#w:lanes) (b:lbytes (w * size_block)) (i:nat{i < w}) : pfelem =
+  nat_from_bytes_le (sub b (i * size_block) size_block)
 
 let load_elem (#w:lanes) (b:lbytes (w * size_block)) : elem w =
-  match w with
-  | 1 -> load_elem1 b
-  | 2 -> load_elem2 b
-  | 4 -> load_elem4 b
+  createi w (load_elem1 #w b)
 
 let load_blocks (#w:lanes) (b:lbytes (w * size_block)) : elem w =
   let e = load_elem #w b in
-  let e = map (pfadd (pow2 128)) e in
-  e
+  map (pfadd (pow2 128)) e
 
-let load_acc1 (text:lbytes size_block) (acc:pfelem) : elem 1 =
-  let acc = create 1 acc in
-  fadd acc (load_blocks #1 text)
+let load_acc (#w:lanes) (text:lbytes (w * size_block)) (acc0:pfelem) : elem w =
+  let acc = create w 0 in
+  let acc = acc.[0] <- acc0 in
+  fadd acc (load_blocks #w text)
 
-let load_acc2 (text:lbytes (2 * size_block)) (acc:pfelem) : elem 2 =
-  let acc = create2 acc 0 in
-  fadd acc (load_blocks #2 text)
+let precomp_rw1 (r:pfelem) : elem 1 =
+  to_elem 1 r
 
-let load_acc4 (text:lbytes (4 * size_block)) (acc:pfelem) : elem 4 =
-  let acc = create4 acc 0 0 0 in
-  fadd acc (load_blocks #4 text)
-
-let load_acc (#w:lanes) (text:lbytes (w * size_block)) (acc:pfelem) : elem w =
-  match w with
-  | 1 -> load_acc1 text acc
-  | 2 -> load_acc2 text acc
-  | 4 -> load_acc4 text acc
-
-let normalize_1 (r:pfelem) (acc:elem 1) : pfelem =
-  pfmul acc.[0] r
-
-let normalize_2 (r:pfelem) (acc:elem 2) : pfelem =
+let precomp_rw2 (r:pfelem) : elem 2 =
   let r2 = pfmul r r in
-  let r21 = create2 r2 r in
-  let a = fmul acc r21 in
-  pfadd a.[0] a.[1]
+  create2 r2 r
 
-let normalize_4 (r:pfelem) (acc:elem 4) : pfelem =
+let precomp_rw4 (r:pfelem) : elem 4 =
   let r2 = pfmul r r in
   let r3 = pfmul r2 r in
   let r4 = pfmul r2 r2 in
-  let r4321 = create4 r4 r3 r2 r in
-  let a = fmul acc r4321 in
-  pfadd (pfadd (pfadd a.[0] a.[1]) a.[2]) a.[3]
+  create4 r4 r3 r2 r
+
+let precomp_rw8 (r:pfelem) : elem 8 =
+  let r2 = pfmul r r in
+  let r3 = pfmul r2 r in
+  let r4 = pfmul r2 r2 in
+  let r5 = pfmul r3 r2 in
+  let r6 = pfmul r4 r2 in
+  let r7 = pfmul r5 r2 in
+  let r8 = pfmul r6 r2 in
+  create8 r8 r7 r6 r5 r4 r3 r2 r
+
+let precomp_rw (#w:lanes) (r:pfelem) : elem w =
+  match w with
+  | 1 -> precomp_rw1 r
+  | 2 -> precomp_rw2 r
+  | 4 -> precomp_rw4 r
+  | 8 -> precomp_rw8 r
+
+let normalize1 (a:elem 1) : pfelem = a.[0]
+let normalize2 (a:elem 2) : pfelem = pfadd a.[0] a.[1]
+let normalize4 (a:elem 4) : pfelem = pfadd (pfadd (pfadd a.[0] a.[1]) a.[2]) a.[3]
+let normalize8 (a:elem 8) : pfelem = pfadd (pfadd (pfadd (pfadd (pfadd (pfadd (pfadd a.[0] a.[1]) a.[2]) a.[3]) a.[4]) a.[5]) a.[6]) a.[7]
 
 let normalize_n (#w:lanes) (r:pfelem) (acc:elem w) : pfelem =
+  let pre = precomp_rw #w r in
+  let acc = fmul acc pre in
   match w with
-  | 1 -> normalize_1 r acc
-  | 2 -> normalize_2 r acc
-  | 4 -> normalize_4 r acc
+  | 1 -> normalize1 acc
+  | 2 -> normalize2 acc
+  | 4 -> normalize4 acc
+  | 8 -> normalize8 acc
 
+// TODO:
+// let pre = precomp_rw #w r in
+// create w pre.[0] == compute_rw #w r
 let compute_r1 (r:pfelem) : elem 1 = to_elem 1 r
 let compute_r2 (r:pfelem) : elem 2 = to_elem 2 (pfmul r r)
 let compute_r4 (r:pfelem) : elem 4 = to_elem 4 (pfmul (pfmul r r) (pfmul r r))
+let compute_r8 (r:pfelem) : elem 8 = to_elem 8 (pfmul (pfmul (pfmul r r) (pfmul r r)) (pfmul (pfmul r r) (pfmul r r)))
 let compute_rw (#w:lanes) (r:pfelem) : elem w =
   match w with
   | 1 -> compute_r1 r
   | 2 -> compute_r2 r
   | 4 -> compute_r4 r
+  | 8 -> compute_r8 r
 
 
 let poly1305_update_nblocks (#w:lanes) (r_w:elem w) (b:lbytes (w * size_block)) (acc:elem w) : elem w =
@@ -126,18 +122,21 @@ let poly1305_update_nblocks (#w:lanes) (r_w:elem w) (b:lbytes (w * size_block)) 
 
 
 let poly1305_update_multi (#w:lanes) (text:bytes{0 < length text /\ length text % (w * size_block) = 0}) (acc:pfelem) (r:pfelem) : pfelem =
-  let rw = compute_rw r in
-  let acc = load_acc (Seq.slice text 0 (w * size_block)) acc in
-  let text = Seq.slice text (w * size_block) (length text) in
-  let acc = repeat_blocks_multi #uint8 #(elem w) (w * size_block) text (poly1305_update_nblocks rw) acc in
-  let acc = normalize_n r acc in
+  let rw = compute_rw #w r in
+  let blocksize_v = w * size_block in
+  let t0 = Seq.slice text 0 blocksize_v in
+  let t1 = Seq.slice text blocksize_v (length text) in
+
+  let acc = load_acc #w t0 acc in
+  let acc = repeat_blocks_multi #uint8 #(elem w) blocksize_v t1 (poly1305_update_nblocks rw) acc in
+  let acc = normalize_n #w r acc in
   acc
 
 
 let poly1305_update_vec (#w:lanes) (text:bytes) (acc:pfelem) (r:pfelem) : pfelem =
   let len = length text in
-  let sz_block = w * size_block in
-  let len0 = len / sz_block * sz_block in
+  let blocksize_v = w * size_block in
+  let len0 = len / blocksize_v * blocksize_v in
   let t0 = Seq.slice text 0 len0 in
   let acc = if len0 > 0 then poly1305_update_multi #w t0 acc r else acc in
 
@@ -150,6 +149,7 @@ let poly1305_update (#w:lanes) (text:bytes) (acc:pfelem) (r:pfelem) : pfelem =
   | 1 -> Scalar.poly1305_update text acc r
   | 2 -> poly1305_update_vec #2 text acc r
   | 4 -> poly1305_update_vec #4 text acc r
+  | 8 -> poly1305_update_vec #8 text acc r
 
 
 let poly1305_mac (#w:lanes) (msg:bytes) (k:Scalar.key) : Scalar.tag =
