code/poly1305/Hacl.Impl.Poly1305.fst
@@ -503,7 +503,7 @@ let poly1305_update32 ctx len text =
 
 
 inline_for_extraction noextract
-val poly1305_update_128_256: #s:field_spec { s = M128 || s = M256 } -> poly1305_update_st s
+val poly1305_update_128_256: #s:field_spec { s = M128 || s = M256 || s = M512} -> poly1305_update_st s
 let poly1305_update_128_256 #s ctx len text =
   let pre = get_precomp_r ctx in
   let acc = get_acc ctx in
