lib/Lib.IntVector.fst
@@ -19,6 +19,7 @@ let vec_t t w =
   | U32,8 -> vec256
   | U64,4 -> vec256
   | U32,16 -> vec512
+  | U64,8 -> vec512
   | _,_ -> admit()
 
 let vec_v #t #w x = admit()
@@ -37,6 +38,7 @@ let vec_zero (t:v_inttype) (w:width) =
   | U64,4
   | U128,2 -> vec256_zero
   | U32,16 -> vec512_zero
+  | U64,8 -> vec512_zero
 
 let vec_counter (t:v_inttype) (w:width) =
   match t,w with
@@ -48,6 +50,7 @@ let vec_counter (t:v_inttype) (w:width) =
   | U64,4 -> vec256_load64s (u64 3) (u64 2) (u64 1) (u64 0)
   | U128,2 -> vec256_load128s (u128 1) (u128 0)
   | U32,16 -> vec512_load32s (u32 15) (u32 14) (u32 13) (u32 12) (u32 11) (u32 10) (u32 9) (u32 8) (u32 7) (u32 6) (u32 5) (u32 4) (u32 3) (u32 2) (u32 1) (u32 0)
+  | U64,8 -> vec512_load64s (u64 7) (u64 6) (u64 5) (u64 4) (u64 3) (u64 2) (u64 1) (u64 0)
 
 let create2 #a x0 x1 = admit()
 let create4 #a x0 x1 x2 x3 = admit()
@@ -65,6 +68,7 @@ let vec_load (#t:v_inttype) (x:uint_t t SEC) (w:width) =
   | U64,4 -> vec256_load64 x
   | U128,2 -> vec256_load128 x
   | U32,16 -> vec512_load32 x
+  | U64,8 -> vec512_load64 x
 
 let vec_load2 #t x1 x0 =
   match t with
@@ -94,7 +98,8 @@ let vec_set (#t:v_inttype) (#w:width) (v:vec_t t w) (i:vec_index w) (x:uint_t t 
   | U8,32 -> vec256_insert8 v x i
   | U32,8 -> vec256_insert32 v x i
   | U64,4 -> vec256_insert64 v x i
-  | U32, 16 -> vec512_insert32 v x i
+  | U32,16 -> vec512_insert32 v x i
+  | U64,8 -> vec512_insert64 v x i
 
 let vec_get (#t:v_inttype) (#w:width) (v:vec_t t w) (i:vec_index w) =
   match t,w with
@@ -106,6 +111,7 @@ let vec_get (#t:v_inttype) (#w:width) (v:vec_t t w) (i:vec_index w) =
   | U32,8 -> vec256_extract32 v i
   | U64,4 -> vec256_extract64 v i
   | U32,16 -> vec512_extract32 v i
+  | U64,8 -> vec512_extract64 v i
 
 let vec_add_mod (#t:v_inttype) (#w:width) (x:vec_t t w) (y:vec_t t w) =
   match t,w with
@@ -116,6 +122,7 @@ let vec_add_mod (#t:v_inttype) (#w:width) (x:vec_t t w) (y:vec_t t w) =
   | U64,4 -> vec256_add64 x y
   | U128,2 -> admit()
   | U32,16 -> vec512_add32 x y
+  | U64,8 -> vec512_add64 x y
 
 let vec_add_mod_lemma (#t:v_inttype) (#w:width) (x:vec_t t w) (y:vec_t t w) = ()
 
@@ -128,6 +135,7 @@ let vec_sub_mod (#t:v_inttype) (#w:width) (x:vec_t t w) (y:vec_t t w) =
   | U64,4 -> vec256_sub64 x y
   | U128,2 -> admit()
   | U32,16 -> vec512_sub32 x y
+  | U64,8 ->  vec512_sub64 x y
 
 
 let vec_mul_mod (#t:v_inttype) (#w:width) (x:vec_t t w) (y:vec_t t w) =
@@ -139,7 +147,7 @@ let vec_mul_mod (#t:v_inttype) (#w:width) (x:vec_t t w) (y:vec_t t w) =
   | U64,4 -> vec256_mul64 x y
   | U128,2 -> admit()
   | U32,16 -> vec512_mul32 x y
-
+  | U64,8 -> vec512_mul64 x y
 
 let vec_smul_mod (#t:v_inttype) (#w:width) (x:vec_t t w) (y:uint_t t SEC) =
   match t,w with
@@ -150,6 +158,7 @@ let vec_smul_mod (#t:v_inttype) (#w:width) (x:vec_t t w) (y:uint_t t SEC) =
   | U64,4 -> vec256_smul64 x y
   | U128,2 -> admit()
   | U32,16 -> vec512_smul32 x y
+  | U64,8 -> vec512_smul64 x y
 
 let vec_xor (#t:v_inttype) (#w:width) (x:vec_t t w) (y:vec_t t w) =
   match t,w with
@@ -163,7 +172,7 @@ let vec_xor (#t:v_inttype) (#w:width) (x:vec_t t w) (y:vec_t t w) =
   | U64,4 -> vec256_xor x y
   | U128,2 -> admit()
   | U32,16 -> vec512_xor x y
-
+  | U64,8 -> vec512_xor x y
 
 let vec_xor_lemma (#t:v_inttype) (#w:width) (x:vec_t t w) (y:vec_t t w) = ()
 
@@ -179,6 +188,7 @@ let vec_and (#t:v_inttype) (#w:width) (x:vec_t t w) (y:vec_t t w) =
   | U64,4 -> vec256_and x y
   | U128,2 -> admit()
   | U32,16 -> vec512_and x y
+  | U64,8 -> vec512_and x y
 
 let vec_and_lemma (#t:v_inttype) (#w:width) (x:vec_t t w) (y:vec_t t w) = ()
 
@@ -194,6 +204,7 @@ let vec_or (#t:v_inttype) (#w:width) (x:vec_t t w) (y:vec_t t w) =
   | U64,4 -> vec256_or x y
   | U128,2 -> admit()
   | U32,16 -> vec512_or x y
+  | U64,8 -> vec512_or x y
 
 let vec_not (#t:v_inttype) (#w:width) (x:vec_t t w) =
   match t,w with
@@ -207,6 +218,7 @@ let vec_not (#t:v_inttype) (#w:width) (x:vec_t t w) =
   | U64,4 -> vec256_lognot x
   | U128,2 -> admit()
   | U32,16 -> vec512_lognot x
+  | U64,8 -> vec512_lognot x
 
 let vec_not_lemma (#t:v_inttype) (#w:width) (x:vec_t t w) = ()
 
@@ -220,6 +232,7 @@ let vec_shift_right (#t:v_inttype) (#w:width) (x:vec_t t w) (y:shiftval t) =
   | U64,4 -> vec256_shift_right64 x y
   | U128,2 -> vec256_shift_right x y
   | U32,16 -> vec512_shift_right32 x y
+  | U64,8 -> vec512_shift_right64 x y
 
 let vec_shift_left (#t:v_inttype) (#w:width) (x:vec_t t w) (y:shiftval t) =
   match t,w with
@@ -231,6 +244,7 @@ let vec_shift_left (#t:v_inttype) (#w:width) (x:vec_t t w) (y:shiftval t) =
   | U64,4 -> vec256_shift_left64 x y
   | U128,2 -> vec256_shift_left x y
   | U32,16 -> vec512_shift_left32 x y
+  | U64,8 -> vec512_shift_left64 x y
 
 let vec_rotate_right (#t:v_inttype) (#w:width) (x:vec_t t w) (y:rotval t) =
   match t,w with
@@ -255,6 +269,7 @@ let vec_eq_mask (#t:v_inttype) (#w:width) (x:vec_t t w) (y:vec_t t w) =
   | U32,8 -> vec256_eq32 x y
   | U64,4 -> vec256_eq64 x y
   | U128,2 -> admit()
+  | U64,8 -> vec512_eq64 x y
 
 let vec_neq_mask (#t:v_inttype) (#w:width) (x:vec_t t w) (y:vec_t t w) =
   vec_not (vec_eq_mask #t #w x y)
@@ -268,6 +283,7 @@ let vec_lt_mask (#t:v_inttype) (#w:width) (x:vec_t t w) (y:vec_t t w) =
   | U32,8 -> vec256_gt32 y x
   | U64,4 -> vec256_gt64 y x
   | U128,2 -> admit()
+  | U64,8 -> vec512_gt64 y x
 
 let vec_gt_mask (#t:v_inttype) (#w:width) (x:vec_t t w) (y:vec_t t w) =
   vec_lt_mask #t #w y x
@@ -290,6 +306,7 @@ let vec_interleave_low_ (#t:v_inttype) (#w:width) (x:vec_t t w) (y:vec_t t w) =
   | U32,16 -> vec512_interleave_low32 x y
   | U64,4 -> vec256_interleave_low64 x y
   | U128,2 -> vec256_interleave_low128 x y
+  | U64,8 -> vec512_interleave_low64 x y
 
 let vec_interleave_low_n (#t:v_inttype) (#w:width) (n:width) (x:vec_t t w) (y:vec_t t w) =
   match t,w,n with
@@ -331,6 +348,7 @@ let vec_interleave_high_ (#t:v_inttype) (#w:width) (x:vec_t t w) (y:vec_t t w) =
   | U32,16 -> vec512_interleave_high32 x y
   | U64,4 -> vec256_interleave_high64 x y
   | U128,2 -> vec256_interleave_high128 x y
+  | U64,8 -> vec512_interleave_high64 x y
 
 let vec_interleave_high_n (#t:v_inttype) (#w:width) (n:width) (x:vec_t t w) (y:vec_t t w) =
   match t,w,n with
@@ -418,6 +436,7 @@ let vec_load_le t w b =
   | U64,4 -> vec256_load_le b
   | U128,2 -> vec256_load_le b
   | U32,16 -> vec512_load_le b
+  | U64,8 -> vec512_load_le b
 
 let vec_load_be t w b =
   match t,w with
@@ -439,6 +458,7 @@ let vec_store_le #t #w b v =
   | U64,4 -> vec256_store_le b v
   | U128,2 -> vec256_store_le b v
   | U32,16 -> vec512_store_le b v
+  | U64,8 -> vec512_store_le b v
 
 let vec_store_be #t #w b v =
   match t,w with
